systems/IDSpace.v
@@ -1,10 +1,3 @@
-Require Bool.Bvector.
-Require Vectors.VectorEq.
-Require Import ZArith.
-Require Zdigits.
-Require Omega.
-Require Import List.
-Import List.ListNotations.
 Require String.
 Require Import StructTact.StructTactics.
 
@@ -15,13 +8,28 @@ Require Import StructTact.StructTactics.
  * operations defined on identifiers are lifted to pointers, which are pairs of
  * a name and the hash of that name, i.e., its identifier. *)
 
-Section IdentifierSpaces.
-  Variable N : nat.
-  Definition id := Bvector.Bvector N.
-  Definition name := String.string.
-  Variable hash : name -> id.
-  Record pointer := mkPointer { ptrId : id;
-                                ptrAddr : name }.
+Definition injective {A B : Type} (f : A -> B) : Prop :=
+  forall a b,
+    f a = f b ->
+    a = b.
+
+Definition name := String.string.
+
+Class IDSpaceParams :=
+  { bits : nat;
+    id : Type;
+    eq_dec :
+      forall a b : id,
+        {a = b} + {a <> b};
+    lt : id -> id -> bool;
+    hash : name -> id;
+    hash_inj : injective hash }.
+
+Section IDSpace.
+  Context `{p : IDSpaceParams}.
+  Record pointer :=
+    mkPointer { ptrId : id;
+                ptrAddr : name }.
 
   Definition make_pointer (n : name) : pointer :=
     {| ptrId := hash n;
@@ -52,7 +60,7 @@ Section IdentifierSpaces.
   Qed.
 
   Definition id_eq_dec : forall a b : id, {a = b} + {a <> b} :=
-    VectorEq.eq_dec _ Bool.eqb Bool.eqb_true_iff _.
+    eq_dec.
 
   Definition pointer_eq_dec : forall x y : pointer,
       {x = y} + {x <> y}.
@@ -62,42 +70,20 @@ Section IdentifierSpaces.
       apply id_eq_dec.
   Defined.
 
-  Definition z_of_id : id -> Z :=
-    Zdigits.binary_value N.
-
-  Definition id_of_z : Z -> id :=
-    Zdigits.Z_to_binary N.
-
-  Lemma z_of_id_inv :
-    forall x,
-      id_of_z (z_of_id x) = x.
-  Proof.
-    unfold id_of_z, z_of_id.
-    apply Zdigits.binary_to_Z_to_binary.
-  Qed.
-
-  Definition bv_ltb (x y : id) : bool :=
-    Z.ltb (z_of_id x) (z_of_id y).
-
   (* true iff x in (a, b) on some sufficiently large "circle" *)
   Definition between_bool (a x b : id) : bool :=
-    match bv_ltb a b, bv_ltb a x, bv_ltb x b with
+    match lt a b, lt a x, lt x b with
     | true, true, true => true
     | false, true, _ => true
     | false, _, true => true
     | _, _, _ => false
     end.
 
-  Lemma bv_ltb_antisymmetric :
+  Lemma lt_antisymmetric :
     forall x y,
-      bv_ltb x y = true ->
-      ~ bv_ltb y x = true.
-  Proof.
-    unfold bv_ltb in *.
-    intros.
-    rewrite Z.ltb_lt in *.
-    omega.
-  Qed.
+      lt x y = true ->
+      ~ lt y x = true.
+  Admitted.
 
   Definition ptr_between_bool (a x b : pointer) : bool :=
     between_bool (ptrId a) (ptrId x) (ptrId b).
@@ -128,7 +114,7 @@ Section IdentifierSpaces.
   Proof.
     unfold between_bool.
     intros.
-    repeat break_if; try find_eapply_lem_hyp bv_ltb_antisymmetric;
+    repeat break_if; try find_eapply_lem_hyp lt_antisymmetric;
       congruence.
   Qed.
 
@@ -150,26 +136,7 @@ Section IdentifierSpaces.
       unroll_between h x y = true ->
       unroll_between h y z = true ->
       unroll_between h x z = true.
-  Proof.
-    unfold unroll_between, between_bool.
-    intros.
-    repeat break_if; try subst; try congruence;
-    unfold bv_ltb in *;
-    rewrite Z.ltb_lt, Z.ltb_nlt in *;
-    omega.
-  Qed.
-
-  Lemma neq_in_id_implies_neq_in_z :
-    forall x y : id,
-      x <> y ->
-      z_of_id x <> z_of_id y.
-  Proof.
-    intros.
-    intro.
-    find_apply_lem_hyp (f_equal id_of_z).
-    repeat rewrite z_of_id_inv in *.
-    congruence.
-  Qed.
+  Admitted.
 
   Lemma unrolling_total :
     forall h x y,
@@ -178,26 +145,14 @@ Section IdentifierSpaces.
   Proof.
     unfold unroll_between, between_bool.
     intros.
-    repeat break_if; try subst; try congruence; auto;
-      unfold bv_ltb in *;
-      try rewrite Z.ltb_lt, Z.ltb_nlt in *;
-      find_apply_lem_hyp neq_in_id_implies_neq_in_z;
-      try omega.
-      rewrite Z.ltb_nlt in *.
-      find_apply_lem_hyp neq_in_id_implies_neq_in_z;
-      try omega.
-  Qed.
+  Admitted.
 
   Lemma unrolling_reflexive :
     forall h x,
       unroll_between h x x = true.
-  Proof.
-    unfold unroll_between, between_bool.
-    intros.
-    repeat break_if; try omega || subst; auto; try congruence.
-  Qed.
+  Admitted.
 
   Definition unroll_between_ptr (h : name) (a b : pointer) :=
     unroll_between (hash h) (ptrId a) (ptrId b).
 
-End IdentifierSpaces.
+End IDSpace.
