extraction/chord/coq/ExtractChord.v
@@ -4,42 +4,21 @@ Require Import ExtrOcamlBasic.
 Require Import Arith Even Div2 EqNat Euclid.
 Require Import ExtrOcamlBasic.
 Require Import ExtrOcamlString.
-
-Extract Inductive nat => int32 [ "0l" "Int32.succ" ]
- "(fun fO fS n -> if n=Int32.zero then fO () else fS (Int32.pred n))".
-
-Extract Constant plus => "(+)".
-Extract Constant pred => "fun n -> Pervasives.max 0l (n-1l)".
-Extract Constant minus => "fun n m -> Pervasives.max 0 (n-m)".
-Extract Constant mult => "( * )".
-Extract Inlined Constant max => "Pervasives.max".
-Extract Inlined Constant min => "Pervasives.min".
-Extract Inlined Constant EqNat.beq_nat => "(=)".
-Extract Inlined Constant EqNat.eq_nat_decide => "(=)".
-
-Extract Inlined Constant Peano_dec.eq_nat_dec => "(=)".
-
-Extract Constant Compare_dec.nat_compare =>
- "fun n m -> if n=m then Eq else if n<m then Lt else Gt".
-Extract Inlined Constant Compare_dec.leb => "(<=)".
-Extract Inlined Constant Compare_dec.le_lt_dec => "(<=)".
-Extract Inlined Constant Compare_dec.lt_dec => "(<)".
-Extract Constant Compare_dec.lt_eq_lt_dec =>
- "fun n m -> if n>m then None else Some (n<m)".
-
-Extract Constant Even.even_odd_dec => "fun n -> Int32.rem n 2 = 0".
-Extract Constant Div2.div2 => "fun n -> Int32.div n 2".
-
-Extract Inductive Euclid.diveucl => "(int * int)" [ "" ].
-Extract Constant Euclid.eucl_dev => "fun n m -> (m/n, m mod n)".
-Extract Constant Euclid.quotient => "fun n m -> m/n".
-Extract Constant Euclid.modulo => "fun n m -> Int32.rem m n".
+Require Import ExtrOcamlNatInt.
 
 Require Import Chord.Chord.
 Import Chord.Chord.Chord.
 
-Extract Inlined Constant Chord.SUCC_LIST_LEN => "3l".
-Extract Constant Chord.hash => "fun n -> Int32.rem n 256l".
+Extract Inlined Constant Chord.SUCC_LIST_LEN => "3".
+
+(* We use the ocaml standard library implementation of MD5 to compute IDs. *)
+Extract Constant Chord.hash => "Digest.of_string".
+(* MD5 digests are 16 bytes. *)
+Extract Inlined Constant Chord.N => "128".
+(* Digest.compare returns -1 if a < b, 0 if a = b, and 1 if a > b *)
+Extract Inlined Constant Chord.id_lt => "(fun a b -> Digest.compare a b < 0)".
+(* id_eq_dec is axiomatized since the entire id type is *)
+Extract Inlined Constant Chord.id_eq_dec => "(=)".
 
 Definition handleNet : addr -> addr -> data -> payload -> res :=
   recv_handler.
